\documentclass[12pt,letterpaper]{article}
\usepackage{preamble}
\usepackage{amsmath}
%%%%%%%%%%%%%%%%%%%%%%%%%%%%%%%%%%%%%%%%%%
%%%% Edit These for yourself
%%%%%%%%%%%%%%%%%%%%%%%%%%%%%%%%%%%%%%%%%%
\newcommand\course{Machine Learning}
\newcommand\userID{Emanuele Belli 03720425 \\ Thomas Brunner 03675118\\ Luca Corbucci 03726968}

\begin{document}.

\section*{Problem 1}

Proof:

$$y = log \sum_{e=1}^N e^{x_i}$$
$$e^y = \sum_{i=1}^N e^{x_i}$$
$$e^{-a}e^{y} = e^{-a}\sum_{i=1}^N e^{x_i}$$
$$e^{y-a} = \sum_{i=1}^N e^{x_i}e^{-a}$$
$$e^{y-a} = \sum_{i=1}^N e^{x_i - a}$$
$$y-a = log\sum_{i=1}^N e^{x_i - a}$$
$$y = a + log\sum_{i=1}^N e^{x_i-a}$$

\section*{Problem 2}

Proof: 

$$\frac{e^{x_i - a}}{\sum_{i=1}^N e^{x_i-a}}=\frac{e^{x_i}e^{-a}}{\sum_{i=1}^N e^{x_1}e^{-a}} $$

$$\frac{e^x_ie^{-a}}{e^{-a}\sum_{i=1}^N e^{x_i}} = \frac{e^{x_i}}{\sum_{i=1}^N e^{x_i}}$$


Alternative Proof:

$$y = \frac{e^{x_i}}{\sum_{i=1}^N e^{x_i}}$$
$$y e^{-a} = \frac{e^{x_i}}{\sum_{i=1}^N e^{x_i}} e^{-a}$$
$$y e^{-a} = \frac{e^{x_i - a}}{\sum_{i=1}^N e^{x_i}}$$
$$y = \frac{e^{x_i-a}}{e^{-a}\sum_{i=1}^N e^{x_i}}$$
$$y = \frac{e^{x_i-a}}{\sum_{i=1}^N e^{x_i-a}}$$
\end{document}